Latest on ctxt equiv proofs

ctxt_equivScript.sml
@@ -35,18 +35,18 @@ Definition plug_def:
     Case x w (rows1 ++ [(v,vs,plug h n)] ++ rows2)
 End
 
-Definition exp_sim_def:
-  exp_sim x y ⇔
+Definition exp_equiv_def:
+  exp_equiv x y ⇔
     ∀bindings.
       set (freevars x) ∪ set (freevars y) ⊆ set (MAP FST bindings) ⇒
       exp_rel (bind bindings x) (bind bindings y)
 End
 
-Theorem exp_sim_closed:
+Theorem exp_equiv_closed:
   closed x ∧ closed y ⇒
-  exp_sim x y = exp_rel x y
+  exp_equiv x y = exp_rel x y
 Proof
-  fs [closed_def,exp_sim_def,bind_def]
+  fs [closed_def,exp_equiv_def,bind_def]
   \\ rw [] \\ eq_tac \\ rw []
   THEN1 (first_x_assum (qspec_then ‘[]’ mp_tac) \\ fs [bind_def])
   \\ fs [GSYM closed_def]
@@ -74,10 +74,10 @@ Proof
   \\ rw [subst_def,bind_def] \\ fs []
 QED
 
-Theorem exp_sim_Lam:
-  exp_sim x y ⇒ exp_sim (Lam s x) (Lam s y)
+Theorem exp_equiv_Lam:
+  exp_equiv x y ⇒ exp_equiv (Lam s x) (Lam s y)
 Proof
-  fs [exp_sim_def] \\ rw []
+  fs [exp_equiv_def] \\ rw []
   \\ fs [bind_Lam]
   \\ rw [] \\ fs []
   \\ fs [exp_rel_def,v_rel_refl,eval_Lam]
@@ -90,16 +90,203 @@ Proof
   \\ metis_tac []
 QED
 
-Theorem exp_sim_plug:
-  ∀h x y. exp_sim x y ⇒ exp_sim (plug h x) (plug h y)
+Inductive similar:
+  (∀x y.
+     exp_rel x y ∧ closed x ∧ closed y ⇒ similar x y)
+  ∧
+  (∀s.
+     similar (Var s) (Var s))
+  ∧
+  (∀f1 f2 x1 x2.
+     similar f1 f2 ∧ similar x1 x2 ⇒
+     similar (App f1 x1) (App f2 x2))
+  ∧
+  (∀s x1 x2.
+     similar x1 x2 ⇒
+     similar (Lam s x1) (Lam s x2))
+  ∧
+  (∀p xs ys.
+     LIST_REL similar xs ys ⇒
+     similar (Prim p xs) (Prim p ys))
+End
+
+Triviality closed_Lam:
+  closed (Lam s1 x1) ∧ closed z ⇒ closed (subst s1 z x1)
+Proof
+  cheat
+QED
+
+Theorem similar_refl[simp]:
+  ∀x. similar x x
+Proof
+  Induct \\ fs []
+  \\ simp [Once similar_cases] \\ fs []
+  \\ cheat (* cases are missing in similar *)
+QED
+
+(* this is the crucial lemma *)
+Theorem similar_Lam_IMP:
+  similar (Lam s1 x1) (Lam s2 x2) ∧ closed z ⇒
+  similar (subst s1 z x1) (subst s2 z x2)
+Proof
+  simp [Once similar_cases] \\ rw []
+  THEN1
+   (simp [Once similar_cases] \\ disj1_tac \\ fs [closed_Lam]
+    \\ last_x_assum mp_tac
+    \\ fs [exp_rel_def,eval_Lam,v_rel_def] \\ rw []
+    \\ first_x_assum (qspec_then ‘SUC n’ mp_tac)
+    \\ fs [v_rel'_def,bind_def]
+    \\ disch_then (qspec_then ‘z’ mp_tac) \\ fs [])
+  \\ qid_spec_tac ‘s1’
+  \\ last_x_assum mp_tac
+  \\ qid_spec_tac ‘x2’
+  \\ qid_spec_tac ‘x1’
+  \\ ho_match_mp_tac similar_strongind
+  \\ rw [] \\ rw []
+  THEN1 (simp [Once similar_cases])
+  THEN1 (fs [subst_def] \\ metis_tac [similar_cases])
+  THEN1 (fs [subst_def] \\ rw [] \\ simp [Once similar_cases])
+  THEN1
+   (simp [Once similar_cases]
+    \\ fs [subst_def] \\ disj2_tac
+    \\ pop_assum mp_tac
+    \\ qid_spec_tac ‘ys’
+    \\ qid_spec_tac ‘xs’
+    \\ Induct \\ fs [PULL_EXISTS])
+QED
+
+(* TODO: the following lemmas about similar probably ought to
+         be proved together *)
+
+Theorem similar_Cons:
+  similar x y ∧ eval x = Constructor s xs ⇒
+  ∃u t. eval x = eval (Cons s t) ∧
+        eval y = eval (Cons s u) ∧ LIST_REL similar t u
+Proof
+  cheat
+QED
+
+Theorem similar_Lam:
+  similar x y ∧ eval x = Closure s z ⇒
+  ∃s1 z1. eval y = Closure s1 z1 ∧ similar (Lam s z) (Lam s1 z1)
+Proof
+  cheat
+QED
+
+Theorem similar_Atom:
+  similar x y ∧ eval x = Atom a ⇒
+  eval y = Atom a
+Proof
+  cheat
+QED
+
+Theorem similar_Diverge:
+  similar x y ∧ eval x = Diverge ⇒
+  eval y = Diverge
+Proof
+  cheat
+QED
+
+Theorem similar_Error:
+  similar x y ∧ eval x = Error ⇒
+  eval y = Error
+Proof
+  cheat
+QED
+
+Theorem similar_imp_exp_equiv:
+  ∀x y. similar x y ⇒ exp_rel x y
+Proof
+  fs [exp_rel_def,v_rel_def,PULL_FORALL,AND_IMP_INTRO]
+  \\ Induct_on ‘n’ \\ fs [v_rel'_def] \\ rw []
+  \\ Cases_on ‘eval x’ \\ fs [] \\ fs [v_rel'_def]
+  THEN1 (drule_all similar_Atom \\ fs [])
+  THEN1
+   (drule_all similar_Cons \\ rw [] \\ fs [eval_Cons]
+    \\ pop_assum mp_tac \\ rename [‘LIST_REL similar xs1 ys1’]
+    \\ qid_spec_tac ‘xs1’ \\ qid_spec_tac ‘ys1’
+    \\ Induct \\ fs [PULL_EXISTS])
+  THEN1
+   (rename [‘Closure s1 x1’]
+    \\ drule_all similar_Lam \\ rw [eval_Lam] \\ rw []
+    \\ rw [] \\ rw [bind_def,v_rel'_refl]
+    \\ imp_res_tac similar_Lam_IMP \\ res_tac)
+  THEN1 (drule_all similar_Diverge \\ fs [])
+  THEN1 (drule_all similar_Error \\ fs [])
+QED
+
+Theorem bind_thm:
+  EVERY closed (MAP SND bs) ⇒
+  bind bs (App x1 x2) = App (bind bs x1) (bind bs x2) ∧
+  bind bs (Prim p xs) = Prim p (MAP (bind bs) xs)
+  (* TODO: add more cases here *)
+Proof
+  cheat
+QED
+
+Theorem bind_fail:
+  ~EVERY closed (MAP SND bs) ⇒ bind bs x = Fail
+Proof
+  cheat
+QED
+
+Theorem closed_bind:
+  set (freevars x) ⊆ set (MAP FST bindings) ⇒ closed (bind bindings x)
+Proof
+  cheat
+QED
+
+Triviality exp_rel_bind_closed:
+  (EVERY closed (MAP SND bs) ⇒
+   exp_rel (bind bs x) (bind bs y)) ⇒
+  exp_rel (bind bs x) (bind bs y)
+Proof
+  Cases_on ‘EVERY closed (MAP SND bs)’
+  \\ full_simp_tac bool_ss [bind_fail,exp_rel_refl]
+QED
+
+Triviality LIST_REL_similar_refl:
+  ∀xs. LIST_REL similar xs xs
+Proof
+  Induct \\ fs []
+QED
+
+Theorem exp_equiv_plug:
+  ∀h x y. exp_equiv x y ⇒ exp_equiv (plug h x) (plug h y)
 Proof
   ho_match_mp_tac plug_ind \\ rw []
   THEN1 (rename [‘Hole’] \\ fs [plug_def])
-  THEN1 (rename [‘Prim’] \\ cheat (* help? *))
-  THEN1 (rename [‘AppL’] \\ cheat (* help? *))
-  THEN1 (rename [‘AppR’] \\ cheat (* help? *))
-  THEN1 (rename [‘Lam’] \\ fs [plug_def,exp_sim_Lam])
-  \\ cheat (* help? *)
+  THEN1 (rename [‘Prim’]
+    \\ rw [exp_equiv_def,plug_def]
+    \\ match_mp_tac exp_rel_bind_closed \\ rw [bind_thm]
+    \\ match_mp_tac similar_imp_exp_equiv
+    \\ simp [Once similar_cases] \\ disj2_tac
+    \\ match_mp_tac rich_listTheory.EVERY2_APPEND_suff
+    \\ fs [LIST_REL_similar_refl]
+    \\ simp [Once similar_cases] \\ disj1_tac
+    \\ fs [closed_bind]
+    \\ first_x_assum drule
+    \\ fs [exp_equiv_def])
+  THEN1 (rename [‘AppL’]
+    \\ rw [exp_equiv_def,plug_def]
+    \\ match_mp_tac exp_rel_bind_closed \\ rw [bind_thm]
+    \\ match_mp_tac similar_imp_exp_equiv
+    \\ simp [Once similar_cases] \\ disj2_tac
+    \\ simp [Once similar_cases] \\ disj1_tac
+    \\ fs [closed_bind]
+    \\ first_x_assum drule
+    \\ fs [exp_equiv_def])
+  THEN1 (rename [‘AppR’]
+    \\ rw [exp_equiv_def,plug_def]
+    \\ match_mp_tac exp_rel_bind_closed \\ rw [bind_thm]
+    \\ match_mp_tac similar_imp_exp_equiv
+    \\ simp [Once similar_cases] \\ disj2_tac
+    \\ simp [Once similar_cases] \\ disj1_tac
+    \\ fs [closed_bind]
+    \\ first_x_assum drule
+    \\ fs [exp_equiv_def])
+  THEN1 (rename [‘Lam’] \\ fs [plug_def,exp_equiv_Lam])
+  \\ cheat (* ... can be done once similar def covers all cases ... *)
 QED
 
 val _ = export_theory();
